src/ursus/CUE/Props_QCTest.v
@@ -95,6 +95,7 @@ CUE_2 (quickFixState {$$
         id updateId code custodianIndex codeHash owners reqConfirms lifetime ? .
 
 (* fails SOMETIMES *)
+
 QuickCheck CUE_2_propb.
 
 Definition CUE_3_propb l id
@@ -150,62 +151,9 @@ CUE_4  (quickFixState {$$
 (* OK *)
 QuickCheck CUE_4_propb.
 
-
-Definition CUE_6_2' l id id2 (updateId :  uint64)  (code : optional cell_) (codeHash : optional uint256) (owners : optional (listArray uint256)) (reqConfirms : optional uint8) (lifetime :  optional   uint32) : Prop := 
-  let l' := exec_state (Uinterpreter (executeUpdate rec def updateId code)) l in
-  let m_updateRequests := toValue (eval_state (sRReader (m_updateRequests_right rec def) ) l) in
-  let res := toValue (eval_state (sRReader (m_updateRequests_right rec def) ) l') in
-  let ur := xMaybeMapDefault (fun x => x) (hmapLookup id m_updateRequests) dummyRequest  in
-  let u2 := xMaybeMapDefault (fun x => x) (hmapLookup id2 res) dummyRequest  in
-  let tr_id := getPruvendoRecord UpdateRequest_ι_id ur in 
-  let tr_id2 := getPruvendoRecord UpdateRequest_ι_id u2 in 
-  let pcode := (toValue (eval_state (sRReader || tvm->code() ) l)) in
-  let ecode := (toValue (eval_state (sRReader || tvm->code() ) l')) in
-  let ccode := (toValue (eval_state (sRReader || tvm->currentCode() ) l')) in
-  let m_custodians := toValue (eval_state (sRReader (m_custodians_right rec def) ) l') in
-  let m_custodians_old := toValue (eval_state (sRReader (m_custodians_right rec def) ) l) in
-  let m_ownerKey_old := toValue (eval_state (sRReader (m_ownerKey_right rec def) ) l) in
-  let m_ownerKey := toValue (eval_state (sRReader (m_ownerKey_right rec def) ) l') in
-  let m_lifetime := toValue (eval_state (sRReader (m_lifetime_right rec def) ) l') in
-  let m_lifetime_old := toValue (eval_state (sRReader (m_lifetime_right rec def) ) l) in
-  let m_defaultRequiredConfirmations := toValue (eval_state (sRReader (m_defaultRequiredConfirmations_right rec def) ) l') in
-  let m_defaultRequiredConfirmations_old := toValue (eval_state (sRReader (m_defaultRequiredConfirmations_right rec def) ) l) in
-  let DEFAULT_LIFETIME := toValue (eval_state (sRReader (DEFAULT_LIFETIME_right rec def) ) l) in
-  let m_requestsMask := toValue (eval_state (sRReader (m_requestsMask_right rec def) ) l') in
-  let m_updateRequestsMask := toValue (eval_state (sRReader (m_updateRequestsMask_right rec def) ) l') in
-  let m_transactions := toValue (eval_state (sRReader (m_transactions_right rec def) ) l') in
-  let m_updateRequests := toValue (eval_state (sRReader (m_updateRequests_right rec def) ) l') in
-  correctState l ->
-  isError (eval_state (Uinterpreter (executeUpdate rec def updateId code)) l) = false -> 
-  (* (u2 <> ur -> hmapIsMember id2 m_updateRequests -> hmapIsMember id2 res) ->
-  length_ m_updateRequests - 1 = length_ res /\
-  tr_id <> tr_id2 /\
-  pcode = ecode /\
-  ccode = ecode /\
-  (xMaybeIsSome owners = true -> length_ (xMaybeMapDefault Datatypes.id owners default) <= length_ m_custodians ) /\
-   checkMap1 m_custodians = true /\
-  checkMap2 m_custodians (N.to_nat (length_ (xMaybeMapDefault Datatypes.id owners default))) (xMaybeMapDefault Datatypes.id owners default) = true /\
-  (xMaybeIsSome owners = false -> m_custodians = m_custodians_old /\ m_ownerKey = m_ownerKey_old) /\
-  xMaybeIsSome reqConfirms = true -> uint2N m_defaultRequiredConfirmations = N.min (length_ m_custodians) (uint2N (xMaybeMapDefault Datatypes.id reqConfirms default)) /\
-  xMaybeIsSome reqConfirms = false -> m_defaultRequiredConfirmations = m_defaultRequiredConfirmations_old /\*)
-  (xMaybeIsSome lifetime = false -> m_lifetime = m_lifetime_old) /\
-  (xMaybeIsSome lifetime = true -> uint2N (xMaybeMapDefault Datatypes.id lifetime default) > 0 -> m_lifetime = (xMaybeMapDefault Datatypes.id lifetime default)) /\
-  (xMaybeIsSome lifetime = true -> uint2N (xMaybeMapDefault Datatypes.id lifetime default) = 0 -> m_lifetime = DEFAULT_LIFETIME) (*/\
-  i >= 0 -> i < 32 ->  N.land (uint2N m_updateRequestsMask) i = 0 /\
-  m_transactions = default /\
-  m_updateRequests = default /\
-  i >= 0 -> i < 32 -> N.land (uint2N m_requestsMask) i = 0*).
-  (* This makes qc freezes XD *)
-  (* i >= 0 -> i < 32 -> N.shiftl (uint2N i) (uint2N m_updateRequestsMask) = 0. *)
-
-
-Definition CUE_6_2_propb l id id2
+Definition CUE_6_2_propb l
         (updateId :  uint64)
         (code : optional cell_) 
-        (codeHash : optional uint256) 
-        (owners : optional (listArray uint256)) 
-        (reqConfirms : optional uint8)
-        (lifetime : optional uint32)
         (mpk: uint256)
         (acc: bool)
         (update: UpdateRequestLRecord)
@@ -217,21 +165,16 @@ let v2 := {$$ v1 with VMState_ι_msg_pubkey := mpk $$} in
 let v3 := {$$ v2 with VMState_ι_now := now $$} in
 let v4 := {$$ v3 with VMState_ι_timestamp := timestamp $$} in
 
-let custodians : XHMap uint256 uint8 := getPruvendoRecord _m_custodians l in
-let custodians' := if hmapIsMember mpk custodians then custodians 
-else xHMapInsert mpk (Build_XUBInteger (length_ custodians)) custodians in
-
 let updates := getPruvendoRecord _m_updateRequests l in
 let updates' := if hmapIsMember updateId updates then updates 
 else xHMapInsert updateId update updates in
 
 
-CUE_6_2'  (quickFixState {$$ 
+CUE_6_2 (quickFixState {$$ 
         {$$ LedgerDefault with Ledger_MainState := 
-        {$$ {$$ l with  _m_custodians := custodians' $$} 
-                  with _m_updateRequests := updates' $$} $$}
+        {$$ l with _m_updateRequests := updates' $$} $$}
                             with Ledger_VMState := v4 $$})
-        id id2 updateId code codeHash owners reqConfirms lifetime ? .
+        updateId code ? .
 
-(* Fail *)
+(* OK *)
 QuickCheck CUE_6_2_propb.
