src/ursus/INT/Props_QCTest.v
@@ -55,12 +55,14 @@ Definition INT_1_propb
        (lifetime :  uint32)
        (mpk: uint256)
        (acc: bool)
-       (pk: uint256): bool :=
+       (pk: uint256)
+       now: bool :=
 let v0 := {$$ VMStateDefault with VMState_ι_msg_pubkey := mpk $$} in     
 let v1 := {$$ v0 with VMState_ι_accepted := acc $$} in
 let v2 := {$$ v1 with VMState_ι_msg_pubkey := pk $$} in
+let v3 := {$$ v2 with VMState_ι_now := Build_XUBInteger (4000 + now) $$} in
 
-INT_1 {$$ LedgerDefault with Ledger_VMState := v2 $$}
+INT_1 {$$ LedgerDefault with Ledger_VMState := v3 $$}
        owners reqConfirms lifetime ? .
 
 (* OK *)
@@ -72,12 +74,14 @@ Definition INT_2_propb
        (lifetime :  uint32)
        (mpk: uint256)
        (acc: bool)
-       (pk: uint256): bool :=
+       (pk: uint256)
+       now: bool :=
 let v0 := {$$ VMStateDefault with VMState_ι_msg_pubkey := mpk $$} in     
 let v1 := {$$ v0 with VMState_ι_accepted := acc $$} in
 let v2 := {$$ v1 with VMState_ι_msg_pubkey := pk $$} in
+let v3 := {$$ v2 with VMState_ι_now := Build_XUBInteger (4000 + now) $$} in
 
-INT_2 {$$ LedgerDefault with Ledger_VMState := v2 $$}
+INT_2 {$$ LedgerDefault with Ledger_VMState := v3 $$}
        owners reqConfirms lifetime ? .
 
 (* OK *)
@@ -87,16 +91,18 @@ Definition INT_3_1_propb l
        (updateId :  uint64)
        (mpk: uint256)
        (acc: bool)
-       (bal: N): bool :=
+       (bal: N)
+       now: bool :=
 let v0 := {$$ VMStateDefault with VMState_ι_msg_pubkey := mpk $$} in     
 let v1 := {$$ v0 with VMState_ι_accepted := acc $$} in
 let v2 := {$$ v1 with VMState_ι_balance := Build_XUBInteger (10 * bal) $$} in
+let v3 := {$$ v2 with VMState_ι_now := Build_XUBInteger (4000 + now) $$} in
 let custodians := CommonInstances.wrap Map (Datatypes.cons (mpk, Build_XUBInteger 0) Datatypes.nil) in
 
 INT_3_1 (quickFixState {$$ 
         {$$ LedgerDefault with Ledger_MainState := 
                 {$$ l with  _m_custodians := custodians $$}
-         $$}with Ledger_VMState := v2 $$})
+         $$}with Ledger_VMState := v3 $$})
        updateId  ? .
 
 (* OK *)
@@ -109,16 +115,18 @@ Definition INT_3_2_propb l
        (lifetime : optional uint32)
        (mpk: uint256)
        (acc: bool)
-       (bal: N): bool :=
+       (bal: N)
+       now: bool :=
 let v0 := {$$ VMStateDefault with VMState_ι_msg_pubkey := mpk $$} in     
 let v1 := {$$ v0 with VMState_ι_accepted := acc $$} in
 let v2 := {$$ v1 with VMState_ι_balance := Build_XUBInteger (10 * bal) $$} in
+let v3 := {$$ v2 with VMState_ι_now := Build_XUBInteger (4000 + now) $$} in
 let custodians := CommonInstances.wrap Map (Datatypes.cons (mpk, Build_XUBInteger 0) Datatypes.nil) in
 
 INT_3_2 (quickFixState {$$ 
         {$$ LedgerDefault with Ledger_MainState := 
                 {$$ l with  _m_custodians := custodians $$}
-         $$}with Ledger_VMState := v2 $$})
+         $$}with Ledger_VMState := v3 $$})
        codeHash owners reqConfirms lifetime ? .
 
 (* OK *)
@@ -128,16 +136,18 @@ Definition INT_3_3_propb l
        (transactionId :  uint64)
        (mpk: uint256)
        (acc: bool)
-       (bal: N): bool :=
+       (bal: N)
+       now: bool :=
 let v0 := {$$ VMStateDefault with VMState_ι_msg_pubkey := mpk $$} in     
 let v1 := {$$ v0 with VMState_ι_accepted := acc $$} in
 let v2 := {$$ v1 with VMState_ι_balance := Build_XUBInteger (10 * bal) $$} in
+let v3 := {$$ v2 with VMState_ι_now := Build_XUBInteger (4000 + now) $$} in
 let custodians := CommonInstances.wrap Map (Datatypes.cons (mpk, Build_XUBInteger 0) Datatypes.nil) in
 
 INT_3_3 (quickFixState {$$ 
         {$$ LedgerDefault with Ledger_MainState := 
                 {$$ l with  _m_custodians := custodians $$}
-         $$}with Ledger_VMState := v2 $$})
+         $$}with Ledger_VMState := v3 $$})
        transactionId  ? .
 
 (* OK *)
@@ -152,16 +162,18 @@ Definition INT_3_4_propb l
        (stateInit :  optional TvmCell)
        (mpk: uint256)
        (acc: bool)
-       (bal: N): bool :=
+       (bal: N)
+       now: bool :=
 let v0 := {$$ VMStateDefault with VMState_ι_msg_pubkey := mpk $$} in     
 let v1 := {$$ v0 with VMState_ι_accepted := acc $$} in
 let v2 := {$$ v1 with VMState_ι_balance := Build_XUBInteger (10 * bal) $$} in
+let v3 := {$$ v2 with VMState_ι_now := Build_XUBInteger (4000 + now) $$} in
 let custodians := CommonInstances.wrap Map (Datatypes.cons (mpk, Build_XUBInteger 0) Datatypes.nil) in
 
 INT_3_4 (quickFixState {$$ 
         {$$ LedgerDefault with Ledger_MainState := 
                 {$$ l with  _m_custodians := custodians $$}
-         $$}with Ledger_VMState := v2 $$})
+         $$}with Ledger_VMState := v3 $$})
        dest value bounce allBalance payload stateInit ? .
 
 (* OK *)
@@ -175,16 +187,18 @@ Definition INT_3_5_propb l
             (payload :  cell_) 
             (mpk: uint256)
             (acc: bool)
-            (bal: N): bool :=
+            (bal: N)
+            now: bool :=
 let v0 := {$$ VMStateDefault with VMState_ι_msg_pubkey := mpk $$} in     
 let v1 := {$$ v0 with VMState_ι_accepted := acc $$} in
 let v2 := {$$ v1 with VMState_ι_balance := Build_XUBInteger (10 * bal) $$} in
+let v3 := {$$ v2 with VMState_ι_now := Build_XUBInteger (4000 + now) $$} in
 let custodians := CommonInstances.wrap Map (Datatypes.cons (mpk, Build_XUBInteger 0) Datatypes.nil) in
 
 INT_3_5 (quickFixState {$$ 
         {$$ LedgerDefault with Ledger_MainState := 
                 {$$ l with  _m_custodians := custodians $$}
-         $$}with Ledger_VMState := v2 $$})
+         $$}with Ledger_VMState := v3 $$})
        dest value bounce flags payload  ? .
 
 (* OK *)
@@ -196,12 +210,14 @@ Definition INT_6_propb
             (lifetime :  uint32)
             (mpk: uint256)
             (acc: bool)
-            (pk: uint256): bool :=
+            (pk: uint256)
+            now: bool :=
 let v0 := {$$ VMStateDefault with VMState_ι_msg_pubkey := mpk $$} in     
 let v1 := {$$ v0 with VMState_ι_accepted := acc $$} in
 let v2 := {$$ v1 with VMState_ι_msg_pubkey := pk $$} in
+let v3 := {$$ v2 with VMState_ι_now := Build_XUBInteger (4000 + now) $$} in
 
-INT_6 {$$ LedgerDefault with Ledger_VMState := v2 $$}
+INT_6 {$$ LedgerDefault with Ledger_VMState := v3 $$}
        owners reqConfirms lifetime ? .
 
 (* OK *)
@@ -212,12 +228,14 @@ Definition INT_7_propb
             (reqConfirms :  uint8)
             (lifetime :  uint32)
             (acc: bool)
-            (pk: uint256): bool :=
+            (pk: uint256)
+            now: bool :=
 let v0 := {$$ VMStateDefault with VMState_ι_msg_pubkey := pk $$} in     
 let v1 := {$$ v0 with VMState_ι_accepted := acc $$} in
 let v2 := {$$ v1 with VMState_ι_msg_pubkey := pk $$} in
+let v3 := {$$ v2 with VMState_ι_now := Build_XUBInteger (4000 + now) $$} in
 
-INT_7 {$$ LedgerDefault with Ledger_VMState := v2 $$}
+INT_7 {$$ LedgerDefault with Ledger_VMState := v3 $$}
        owners reqConfirms lifetime ? .
 
 (* OK *)
@@ -228,12 +246,14 @@ Definition INT_8_1_propb
             (reqConfirms :  uint8)
             (lifetime :  uint32)
             (acc: bool)
-            (pk: uint256): bool :=
+            (pk: uint256)
+            now: bool :=
 let v0 := {$$ VMStateDefault with VMState_ι_msg_pubkey := pk $$} in     
 let v1 := {$$ v0 with VMState_ι_accepted := acc $$} in
 let v2 := {$$ v1 with VMState_ι_pubkey := pk $$} in
+let v3 := {$$ v2 with VMState_ι_now := Build_XUBInteger (4000 + now) $$} in
 
-INT_8_1 {$$ LedgerDefault with Ledger_VMState := v2 $$}
+INT_8_1 {$$ LedgerDefault with Ledger_VMState := v3 $$}
        owners reqConfirms lifetime ? .
 
 (* OK *)
